theories/microgv/invariant.v
@@ -1,0 +1,71 @@
+From diris.microgv Require Export rtypesystem.
+
+Definition linv (ρ : cfg) (v : vertex) (in_l : multiset label) : rProp :=
+  match v with
+  | VThread k =>
+    ⌜⌜ in_l ≡ ε ⌝⌝ ∗
+    match ρ !! k with
+    | Some (Thread e) => rtyped0 e UnitT
+    | _ => emp
+    end
+  | VBarrier k =>
+    ⌜⌜ match ρ !! k with
+      | Some Barrier => ∃ t1 t2, in_l ≡ {[ (t1,t2)]} ⋅ {[ (t2,t1) ]}
+      | _ => in_l ≡ ε
+      end ⌝⌝
+  end%I.
+
+Definition ginv ρ := inv (linv ρ).
+
+Lemma lookup_union_spec `{Countable K} {V} (m1 m2 : gmap K V) (x : K) :
+  (m1 ∪ m2) !! x = from_option Some (m2 !! x) (m1 !! x).
+Proof.
+  rewrite lookup_union.
+  destruct (m1 !! x),(m2 !! x); simpl; eauto.
+Qed.
+
+Ltac sdec := repeat (progress simp || case_decide || done || eauto).
+Ltac smap := repeat (
+  rewrite lookup_union_spec ||
+  rewrite lookup_alter_spec ||
+  rewrite lookup_insert_spec ||
+  rewrite lookup_delete_spec ||
+  rewrite lookup_empty || sdec).
+
+Lemma preservation i ρ ρ' :
+  step i ρ ρ' -> ginv ρ -> ginv ρ'.
+Proof.
+  intros H Hinv.
+  destruct H as [ρ ρ' ρf D1 D2 i H].
+  destruct H.
+  - eapply inv_impl; last done.
+    iIntros ([n|n] x) "H"; smap.
+    iDestruct "H" as "[? H]". iFrame.
+    iDestruct (replacement with "H") as (t) "[H Q]"; first done.
+    iApply "Q". iApply pure_preservation; done.
+  - eapply inv_impl; last done.
+    iIntros ([n|n] x) "H"; smap; iDestr "H";
+    assert (ρf !! n = None) as -> by solve_map_disjoint; eauto.
+    destruct v; simpl; iDestr "H"; simp. done.
+  - eapply (inv_alloc_lr (VThread i0) (VBarrier n) (VThread j)); last done; first admit; first admit.
+    + naive_solver.
+    + iIntros (? ? ?) "H". simp.
+      destruct v0; simpl; smap;
+      assert (ρf !! n0 = None) as -> by solve_map_disjoint; eauto.
+    + iIntros (?) "H". simpl. smap.
+      assert (ρf !! n = None) as -> by solve_map_disjoint; eauto.
+    + iIntros (?) "H". simpl. smap. iDestr "H".
+      assert (ρf !! j = None) as -> by solve_map_disjoint; eauto.
+    + iIntros (?) "H". simpl.
+      iDestr "H". rewrite lookup_union_spec lookup_singleton. simpl.
+      iDestruct (replacement with "H") as (t) "[H Q]"; first done. simpl.
+      iDestr "H". simp.
+      iExists (t1,t2), (t2,t1).
+      iSplitL "Q".
+      * smap. iIntros "H". iSplit; first done.
+        iApply "Q". simpl. iSpl; eauto.
+      * smap. iSplit; eauto.
+        iIntros "Q". iSplit; eauto.
+        iSpl. iFrame. iSpl; eauto.
+  - admit.
+Admitted.
