theories/microgv/langtools.v
@@ -3,5 +3,6 @@ From diris.cgraphs Require Export util.
 From Coq.Logic Require Export FunctionalExtensionality Classical.
 From diris Require Export seplogic.
 From stdpp Require Export gmap.
+Require Export diris.cgraphs.genericinv.
 
 Ltac inv H := inversion H; clear H; simplify_eq.
