theories/microgv/progress.v
@@ -1,0 +1,27 @@
+From diris.microgv Require Export invariant.
+
+Definition vertex_waiting (ρ : cfg) (x y : vertex) (l : label) :=
+  match x,y with
+  | VThread n, VBarrier k => True
+  | _,_ => False
+  end.
+
+Definition vertex_reachable ρ (v : vertex) :=
+  match v with
+  | VThread n => reachable ρ n
+  | VBarrier n => reachable ρ n
+  end.
+
+Lemma full_reachability ρ :
+  ginv ρ -> fully_reachable ρ.
+Proof.
+  unfold fully_reachable.
+  intros Hinv i.
+  classical_right.
+  destruct Hinv as [g [Hwf Hinv]].
+  cut (∀ v, vertex_reachable ρ v). admit.
+  intros v.
+  eapply (cgraph_ind' (vertex_waiting ρ) g (vertex_reachable ρ)); eauto; first admit.
+  intros.
+    [solve_proper|eauto|].
+Admitted.
